theories/ftlr/Subseg.v
@@ -114,7 +114,7 @@ Section fundamental.
         iDestruct (region_close with "[$Hstate $Hr $Ha $Hmono]") as "Hr"; eauto.
         { destruct ρ;auto;[..|specialize (Hnotstatic g)];contradiction. }
         iApply ("IH" $! _ r with "[%] [] [Hmap] [$Hr] [$Hsts] [$Hown]"); try iClear "IH"; eauto.
-        iAlways. 
+        iModIntro. 
         generalize (isWithin_implies _ _ _ _ H4). intros [A B].
         destruct (Z_le_dec b'' e'').
         + rewrite (isWithin_region_addrs_decomposition b'' e'' b0 e0); auto.
