theories/multiple_updates.v
@@ -1,10 +1,10 @@
 From iris.proofmode Require Import tactics.
 From cap_machine Require Export region_invariants_revocation.
-From cap_machine Require Import logrel. 
+From cap_machine Require Import logrel.
 Require Import Eqdep_dec List.
 From stdpp Require Import countable.
 
-Section std_updates. 
+Section std_updates.
 
   (* --------------------------------------------------------------------------------- *)
   (* ----------------------- UPDATING MULTIPLE REGION STATES ------------------------- *)
@@ -15,49 +15,49 @@ Section std_updates.
 
   Notation STS := (leibnizO (STS_states * STS_rels)).
   Notation STS_STD := (leibnizO (STS_std_states Addr region_type)).
-  Notation WORLD := (prodO STS_STD STS). 
+  Notation WORLD := (prodO STS_STD STS).
   Implicit Types W : WORLD.
-  
+
   Fixpoint std_update_multiple W l ρ :=
     match l with
     | [] => W
     | a :: l => std_update (std_update_multiple W l ρ) a ρ
     end.
-   
+
    Definition std_update_temp_multiple W l := std_update_multiple W l Temporary.
 
    Lemma std_update_multiple_loc_sta W l ρ :
      (std_update_multiple W l ρ).2.1 = W.2.1.
    Proof.
-     induction l; auto. 
-   Qed.      
+     induction l; auto.
+   Qed.
 
    Lemma std_update_multiple_loc_rel W l ρ :
      (std_update_multiple W l ρ).2.2 = W.2.2.
    Proof.
-     induction l; auto. 
+     induction l; auto.
    Qed.
 
    Lemma std_update_multiple_loc W l ρ :
-     (std_update_multiple W l ρ).2 = W.2. 
+     (std_update_multiple W l ρ).2 = W.2.
    Proof.
-     induction l; auto. 
+     induction l; auto.
    Qed.
 
    Lemma std_update_multiple_proj_eq W Wloc l ρ :
      ((std_update_multiple W l ρ).1, Wloc) = std_update_multiple (W.1,Wloc) l ρ.
    Proof.
-     destruct W as [Wsta Wloc']. simpl. induction l; auto. 
+     destruct W as [Wsta Wloc']. simpl. induction l; auto.
      simpl. rewrite -IHl. auto.
    Qed.
 
    Lemma std_update_multiple_std_sta_eq W Wloc l ρ :
      (std_update_multiple W l ρ).1 = (std_update_multiple (W.1, Wloc) l ρ).1.
    Proof.
-     destruct W as [Wsta Wloc']. simpl. induction l; auto. 
+     destruct W as [Wsta Wloc']. simpl. induction l; auto.
      simpl. rewrite -IHl. auto.
    Qed.
-   
+
    Lemma std_update_multiple_swap_head W l a1 a2 ρ :
      std_update_multiple W (a1 :: a2 :: l) ρ = std_update_multiple W (a2 :: a1 :: l) ρ.
    Proof.
@@ -69,13 +69,13 @@ Section std_updates.
      - destruct (decide (a1 = a2)); subst;[done|].
        simpl. rewrite /std_update.
        repeat rewrite (insert_commute _ a1 a2) ; auto.
-   Qed. 
-       
+   Qed.
+
    Lemma std_update_multiple_swap W l1 a l2 ρ :
      std_update_multiple W (l1 ++ a :: l2) ρ = std_update_multiple W (a :: l1 ++ l2) ρ.
    Proof.
      induction l1; auto.
-     rewrite app_comm_cons std_update_multiple_swap_head /=. 
+     rewrite app_comm_cons std_update_multiple_swap_head /=.
      f_equal;auto.
    Qed.
 
@@ -84,10 +84,10 @@ Section std_updates.
      l1 ≡ₚ l2 →
      std_update_multiple W l1 ρ = std_update_multiple W l2 ρ.
    Proof.
-     intros Hperm. 
+     intros Hperm.
      induction Hperm using Permutation_ind.
      - done.
-     - simpl. rewrite IHHperm. done. 
+     - simpl. rewrite IHHperm. done.
      - apply (std_update_multiple_swap_head W l y x).
      - by rewrite IHHperm1 IHHperm2.
    Qed.
@@ -96,10 +96,10 @@ Section std_updates.
      Proper (Permutation ==> eq) (λ l, std_update_multiple W l ρ).
    Proof. intros y1 y2 Hperm. simpl. by apply std_update_multiple_permutation. Defined.
 
-   
+
    Lemma remove_dups_swap_head {A : Type} `{EqDecision A} (a1 a2 : A) (l : list A) :
      remove_dups (a1 :: a2 :: l) ≡ₚ remove_dups (a2 :: a1 :: l).
-   Proof. 
+   Proof.
      destruct (decide (a1 = a2)); subst; auto.
      simpl. destruct (decide_rel elem_of a1 (a2 :: l)), (decide_rel elem_of a2 (a1 :: l)).
      - apply elem_of_cons in e as [Hcontr | Hl];[subst;contradiction|].
@@ -108,22 +108,22 @@ Section std_updates.
        destruct (decide_rel elem_of a1 l);[|contradiction].
        done.
      - apply elem_of_cons in e as [Hcontr | Hl];[subst;contradiction|].
-       apply not_elem_of_cons in n0 as [Hcontr Hl0]. 
+       apply not_elem_of_cons in n0 as [Hcontr Hl0].
        destruct (decide_rel elem_of a2 l);[contradiction|].
        destruct (decide_rel elem_of a1 l);[|contradiction].
        done.
      - apply elem_of_cons in e as [Hcontr | Hl];[subst;contradiction|].
-       apply not_elem_of_cons in n0 as [Hcontr Hl0]. 
+       apply not_elem_of_cons in n0 as [Hcontr Hl0].
        destruct (decide_rel elem_of a2 l);[|contradiction].
        destruct (decide_rel elem_of a1 l);[contradiction|].
        done.
-     - apply not_elem_of_cons in n1 as [Hcontr Hl]. 
-       apply not_elem_of_cons in n0 as [Hcontr0 Hl0]. 
-       destruct (decide_rel elem_of a2 l); [contradiction|]. 
+     - apply not_elem_of_cons in n1 as [Hcontr Hl].
+       apply not_elem_of_cons in n0 as [Hcontr0 Hl0].
+       destruct (decide_rel elem_of a2 l); [contradiction|].
        destruct (decide_rel elem_of a1 l);[contradiction|].
-       rewrite (Permutation_swap a1 a2 (remove_dups l)). done. 
-   Qed. 
-     
+       rewrite (Permutation_swap a1 a2 (remove_dups l)). done.
+   Qed.
+
    Lemma remove_dups_swap {A : Type} `{EqDecision A} (l1 : list A) (a : A) (l2 : list A) :
      remove_dups (l1 ++ a :: l2) ≡ₚremove_dups (a :: l1 ++ l2).
    Proof.
@@ -131,12 +131,12 @@ Section std_updates.
      rewrite app_comm_cons remove_dups_swap_head (app_comm_cons l1 l2 a) /=.
      destruct (decide_rel elem_of a0 (l1 ++ a :: l2)).
      - rewrite decide_True;[|by rewrite Permutation_middle].
-       destruct (decide_rel elem_of a (l1 ++ l2)). 
-       + rewrite IHl1. simpl. rewrite decide_True; auto. 
+       destruct (decide_rel elem_of a (l1 ++ l2)).
+       + rewrite IHl1. simpl. rewrite decide_True; auto.
        + rewrite IHl1. simpl. rewrite decide_False; auto.
-     - rewrite decide_False;[|by rewrite Permutation_middle]. f_equiv. 
-       destruct (decide_rel elem_of a (l1 ++ l2)). 
-       + rewrite IHl1. simpl. rewrite decide_True; auto. 
+     - rewrite decide_False;[|by rewrite Permutation_middle]. f_equiv.
+       destruct (decide_rel elem_of a (l1 ++ l2)).
+       + rewrite IHl1. simpl. rewrite decide_True; auto.
        + rewrite IHl1. simpl. rewrite decide_False; auto.
    Qed.
 
@@ -166,7 +166,7 @@ Section std_updates.
      apply elem_of_cons in Hnin as [Hne | Hnin].
      - subst i. rewrite lookup_insert; auto.
      - destruct (decide (a = i));[subst i; rewrite lookup_insert; auto|].
-       rewrite lookup_insert_ne;auto. 
+       rewrite lookup_insert_ne;auto.
    Qed.
 
    (* ------------------------------------------------------------ *)
@@ -179,14 +179,14 @@ Section std_updates.
      destruct (decide (i ∈ l)).
      - exists ρ. by apply std_sta_update_multiple_lookup_in_i.
      - rewrite std_sta_update_multiple_lookup_same_i;auto.
-   Qed. 
+   Qed.
 
    (* ------------------------------------------------------------ *)
-   
+
    (* domains *)
    Lemma std_update_multiple_not_in_sta_i W l ρ i :
      i ∉ l → i ∈ dom (gset Addr) (std W) ↔
-               i ∈ dom (gset Addr) (std (std_update_multiple W l ρ)). 
+               i ∈ dom (gset Addr) (std (std_update_multiple W l ρ)).
    Proof.
      intros Hnin. induction l; auto.
      apply not_elem_of_cons in Hnin as [Hneq Hnin].
@@ -206,12 +206,12 @@ Section std_updates.
    Lemma std_update_multiple_not_in_sta W l ρ (a : Addr) :
      a ∉ l → a ∈ dom (gset Addr) (std W) ↔
              a ∈ dom (gset Addr) (std (std_update_multiple W l ρ)).
-   Proof. 
+   Proof.
      intros Hnin.
-     apply std_update_multiple_not_in_sta_i. 
+     apply std_update_multiple_not_in_sta_i.
      intros Hcontr. contradiction.
    Qed.
-   
+
    (* ---------------------------------------------------------------------------- *)
    (* Some helper lemmas for various lemmas about using multiple updates in region *)
 
@@ -220,7 +220,7 @@ Section std_updates.
      related_sts_pub_world W (std_update_multiple W l ρ).
    Proof.
      intros Hforall. induction l.
-     - apply related_sts_pub_refl_world. 
+     - apply related_sts_pub_refl_world.
      - simpl.
        apply list.Forall_cons in Hforall as [ Ha_std Hforall].
        eapply related_sts_pub_trans_world;[apply IHl; auto|].
@@ -240,31 +240,31 @@ Section std_updates.
      intros Helem.
      apply elem_of_list_lookup_2 in Helem.
      apply elem_of_list_split in Helem as [l1 [l2 Heq] ].
-     rewrite Heq std_update_multiple_swap /= /std_update. 
-     rewrite /std /=. rewrite lookup_insert. auto. 
-   Qed. 
-   
+     rewrite Heq std_update_multiple_swap /= /std_update.
+     rewrite /std /=. rewrite lookup_insert. auto.
+   Qed.
+
    Lemma std_update_temp_multiple_lookup W l k y :
      l !! k = Some y →
      region_state_pwl (std_update_temp_multiple W l) y.
    Proof.
-     apply std_update_multiple_lookup. 
+     apply std_update_multiple_lookup.
    Qed.
-   
+
 
    (* Multiple updates does not change dom, as long as the updated elements are a subset of original dom *)
    Lemma std_update_multiple_dom_equal W l ρ :
      (∀ i : Addr, i ∈ l → i ∈ dom (gset Addr) (std W)) ->
-     dom (gset Addr) (std W) = dom (gset Addr) (std (std_update_multiple W l ρ)). 
+     dom (gset Addr) (std W) = dom (gset Addr) (std (std_update_multiple W l ρ)).
    Proof.
      intros Hsub.
-     induction l; auto. 
+     induction l; auto.
      rewrite /= /std_update.
      rewrite dom_insert_L.
      assert (a ∈ a :: l) as Hin.
      { apply elem_of_cons. by left. }
      pose proof (Hsub _ Hin) as Hain. etrans;[apply IHl|].
-     - intros i Hi. apply Hsub. apply elem_of_cons. by right. 
+     - intros i Hi. apply Hsub. apply elem_of_cons. by right.
      - set_solver.
    Qed.
 
@@ -283,21 +283,21 @@ Section std_updates.
      dom (gset Addr) (std W) ⊆ dom (gset Addr) (std W') ->
      dom (gset Addr) (std (std_update_multiple W l ρ)) ⊆ dom (gset Addr) (std (std_update_multiple W' l ρ)).
    Proof.
-     induction l;auto. 
+     induction l;auto.
      simpl. repeat rewrite dom_insert_L. set_solver.
    Qed.
-     
+
    Lemma std_update_mutiple_related_monotone W W' l ρ :
      related_sts_pub_world W W' ->
      related_sts_pub_world (std_update_multiple W l ρ) (std_update_multiple W' l ρ).
    Proof.
      intros Hrelated.
      destruct W as [ Wstd_sta [Wloc_sta Wloc_rel] ].
-     destruct W' as [ Wstd_sta' [Wloc_sta' Wloc_rel'] ]. 
+     destruct W' as [ Wstd_sta' [Wloc_sta' Wloc_rel'] ].
      destruct Hrelated as [ [Hstd_dom1 Hstd_related ] Hloc_related].
      simpl in *.
      split;[clear Hloc_related|by repeat rewrite std_update_multiple_loc_rel std_update_multiple_loc_sta].
-     split. 
+     split.
      - apply std_update_multiple_std_sta_dom_monotone. auto.
      - intros i x y Hx Hy.
        destruct (decide (i ∈ l)).
@@ -306,48 +306,48 @@ Section std_updates.
          inversion Hx; inversion Hy; subst. left.
        + rewrite std_sta_update_multiple_lookup_same_i /std /= in Hx;auto.
          rewrite std_sta_update_multiple_lookup_same_i /std /= in Hy;auto.
-         apply Hstd_related with i; auto. 
-   Qed. 
- 
+         apply Hstd_related with i; auto.
+   Qed.
+
    (* lemmas for updating a repetition of top *)
    Lemma std_update_multiple_dom_top_sta W n ρ a :
-     a ≠ top ->
+     a ≠ addr_reg.top ->
      a ∉ dom (gset Addr) (std W) →
-     a ∉ dom (gset Addr) (std (std_update_multiple W (repeat top n) ρ)).
+     a ∉ dom (gset Addr) (std (std_update_multiple W (repeat addr_reg.top n) ρ)).
    Proof.
      intros Hne Hnin.
      induction n; auto.
      simpl. rewrite dom_insert. apply not_elem_of_union.
      split.
      + apply not_elem_of_singleton.
-       intros Hcontr. done. 
+       intros Hcontr. done.
      + apply IHn.
    Qed.
 
    Lemma region_addrs_aux_top n :
-     region_addrs_aux top n = repeat top n.
+     region_addrs_aux addr_reg.top n = repeat addr_reg.top n.
    Proof.
      induction n; auto.
      simpl. f_equiv. done.
-   Qed. 
+   Qed.
 
    Lemma std_update_multiple_dom_sta_i W n ρ a i :
-     a ≠ top → (i > 0)%Z →
+     a ≠ addr_reg.top → (i > 0)%Z →
      a ∉ dom (gset Addr) (std W) →
      a ∉ dom (gset Addr) (std (std_update_multiple W (region_addrs_aux (get_addr_from_option_addr (a + i)%a) n) ρ)).
    Proof.
-     intros Hneq Hgt. 
+     intros Hneq Hgt.
      destruct (a + i)%a eqn:Hsome.
      - simpl.
        assert (a < a0)%a as Hlt;[apply next_lt_i with i; auto|].
        intros Hnin.
-       revert Hlt Hsome. generalize i a0. induction n; auto; intros j a1 Hlt Hsome. 
+       revert Hlt Hsome. generalize i a0. induction n; auto; intros j a1 Hlt Hsome.
        simpl. rewrite dom_insert. apply not_elem_of_union.
        split.
        + apply not_elem_of_singleton.
-         intros Hcontr. subst. rewrite /lt_addr in Hlt. lia.  
-       + destruct (a1 + 1)%a eqn:Ha2; simpl. 
-         ++ apply IHn with (j + 1)%Z. 
+         intros Hcontr. subst. rewrite /lt_addr in Hlt. lia.
+       + destruct (a1 + 1)%a eqn:Ha2; simpl.
+         ++ apply IHn with (j + 1)%Z.
             +++ apply next_lt in Ha2. rewrite /lt_addr in Hlt. rewrite /lt_addr. lia.
             +++ apply (incr_addr_trans a a1 a2 j 1) in Hsome; auto.
          ++ rewrite region_addrs_aux_top. apply std_update_multiple_dom_top_sta; auto.
@@ -371,7 +371,7 @@ Section std_updates.
      std (std_update_multiple (std_update W a' i) (region_addrs a b) ρ) !! l =
      std (std_update (std_update_multiple W (region_addrs a b) ρ) a' i) !! l.
    Proof.
-     intros Hlt. 
+     intros Hlt.
      destruct (decide (l ∈ region_addrs a b)).
      - assert (l ≠ a') as Hne.
        { intros ->. apply region_addrs_not_elem_of with _ (region_size a b) _ in Hlt.
@@ -382,15 +382,15 @@ Section std_updates.
        assert (std (std_update_multiple (std_update W a' i) (region_addrs a b) ρ) !! l = Some ρ) as Hpwl'.
        { apply std_update_multiple_lookup with n. auto. }
        rewrite /region_state_pwl /= in Hpwl. rewrite /region_state_pwl /= in Hpwl'.
-       rewrite -Hpwl in Hpwl'. rewrite Hpwl'. 
-       rewrite lookup_insert_ne; auto. 
-     - rewrite std_sta_update_multiple_lookup_same_i; auto. 
+       rewrite -Hpwl in Hpwl'. rewrite Hpwl'.
+       rewrite lookup_insert_ne; auto.
+     - rewrite std_sta_update_multiple_lookup_same_i; auto.
        destruct (decide ( a' =  l)).
        + rewrite /std_update /std /= e. do 2 rewrite lookup_insert. done.
        + rewrite /std_update /std /=. rewrite lookup_insert_ne;auto. rewrite lookup_insert_ne; auto.
          rewrite std_sta_update_multiple_lookup_same_i; auto.
    Qed.
-       
+
    Lemma std_update_multiple_dom_insert W (a b a' : Addr) i :
      (a' < a)%a →
      Forall (λ a : Addr,
@@ -398,8 +398,8 @@ Section std_updates.
      Forall (λ a : Addr,
                    (a ∉ dom (gset Addr) (<[ a' := i]> W.1))) (region_addrs a b).
    Proof.
-     intros Hlt. 
-     do 2 (rewrite list.Forall_forall). intros Hforall.  
+     intros Hlt.
+     do 2 (rewrite list.Forall_forall). intros Hforall.
      intros x Hin.
      assert (x ≠ a') as Hne.
      { intros Hcontr; subst.
@@ -408,8 +408,8 @@ Section std_updates.
      apply Hforall with x in Hin.
      rewrite dom_insert. apply not_elem_of_union.
      split;auto. apply not_elem_of_singleton.
-     intros Hcontr. contradiction. 
-   Qed. 
+     intros Hcontr. contradiction.
+   Qed.
 
    (* commuting updates and revoke *)
 
@@ -419,14 +419,14 @@ Section std_updates.
    Proof.
      intros Hne.
      induction l; auto; simpl.
-     rewrite IHl. 
+     rewrite IHl.
      rewrite /std_update /revoke /loc /std /=. repeat f_equiv.
      eapply (map_leibniz (M:=gmap Addr) (A:=region_type)). intros i. apply leibniz_equiv_iff.
      destruct (decide (a = i)).
      - subst. rewrite lookup_insert revoke_monotone_lookup_same;rewrite lookup_insert; auto.
-       intros Hcontr; inversion Hcontr as [Hcontr']. done. 
+       intros Hcontr; inversion Hcontr as [Hcontr']. done.
      - rewrite lookup_insert_ne;auto.
-       apply revoke_monotone_lookup. rewrite lookup_insert_ne;auto. Unshelve. apply _. 
+       apply revoke_monotone_lookup. rewrite lookup_insert_ne;auto. Unshelve. apply _.
    Qed.
 
    (* std_update_multiple and app *)
@@ -435,8 +435,8 @@ Section std_updates.
      std_update_multiple W (l1 ++ l2) ρ = std_update_multiple (std_update_multiple W l1 ρ) l2 ρ.
    Proof.
      induction l2; auto.
-     - by rewrite app_nil_r /=. 
-     - rewrite std_update_multiple_swap /=. f_equal. auto. 
+     - by rewrite app_nil_r /=.
+     - rewrite std_update_multiple_swap /=. f_equal. auto.
    Qed.
 
    Lemma std_update_multiple_app_commute W (l1 l2 : list Addr) ρ :
@@ -444,24 +444,25 @@ Section std_updates.
    Proof.
      induction l2.
      - by rewrite app_nil_r /=.
-     - rewrite std_update_multiple_swap /=. by rewrite IHl2. 
+     - rewrite std_update_multiple_swap /=. by rewrite IHl2.
    Qed.
 
    (* Helper lemmas about permutation *)
 
-   Lemma elements_permutation A C `{Empty C, Union C, Singleton A C, Elements A C,ElemOf A C, EqDecision A, FinSet A C} (l: list A) :
-     NoDup l ->
-     elements (list_to_set l) ≡ₚl.
-   Proof. 
-     intros Hdup.
-     induction l. 
-     - by rewrite /= elements_empty. 
-     - apply NoDup_cons_iff in Hdup as [Hnin Hdup].
-       rewrite /= elements_union_singleton; auto. 
-       apply not_elem_of_list_to_set.
-       intros Hcontr. apply elem_of_list_In in Hcontr.
-       done.
-   Qed.
+   (* TODO: never used ? *)
+   (* Lemma elements_permutation A C `{Empty C, Union C, Singleton A C, Elements A C,ElemOf A C, EqDecision A, FinSet A C} (l: list A) : *)
+   (*   NoDup l -> *)
+   (*   elements (list_to_set l) ≡ₚl. *)
+   (* Proof. *)
+   (*   intros Hdup. *)
+   (*   induction l. *)
+   (*   - by rewrite /= elements_empty. *)
+   (*   - apply NoDup_cons_iff in Hdup as [Hnin Hdup]. *)
+   (*     rewrite /= elements_union_singleton; auto. *)
+   (*     apply not_elem_of_list_to_set. *)
+   (*     intros Hcontr. apply elem_of_list_In in Hcontr. *)
+   (*     done. *)
+   (* Qed. *)
 
    (* multiple updates and private relation *)
    Lemma rtc_rel_priv x y:
@@ -477,18 +478,18 @@ Section std_updates.
          | _ => idtac
          end).
   Qed.
-  
+
   Lemma related_sts_priv_world_std_update_multiple W l ρ :
     Forall (λ a : Addr, ∃ ρ, (std W) !! a = Some ρ /\ ρ <> Permanent) l →
     related_sts_priv_world W (std_update_multiple W l ρ).
   Proof.
     intros Hforall.
-    induction l. 
-    - apply related_sts_priv_refl_world. 
+    induction l.
+    - apply related_sts_priv_refl_world.
     - eapply related_sts_priv_trans_world;[apply IHl|].
-      + apply Forall_cons_1 in Hforall as [_ Hforall]. auto. 
+      + apply Forall_cons_1 in Hforall as [_ Hforall]. auto.
       + split;[|rewrite std_update_multiple_loc_rel;apply related_sts_priv_refl].
-        split. 
+        split.
         ++ rewrite /std_update dom_insert_L. set_solver.
         ++ intros j x0 y Hx0 Hy.
            destruct (decide (a = j)).
@@ -503,5 +504,5 @@ Section std_updates.
                eapply rtc_rel_priv; auto.
            +++ rewrite /= lookup_insert_ne in Hy;auto. rewrite Hx0 in Hy; inversion Hy; subst; left.
   Qed.
-     
+
 End std_updates.
