theories/rules/rules_Jmp.v
@@ -33,7 +33,7 @@ Section cap_lang_rules.
   Proof.
     iIntros (Hinstr Hfl Hvpc ϕ) "(>HPC & >Hpc_a & >Hr) Hφ".
     iApply wp_lift_atomic_head_step_no_fork; auto.
-    iIntros (σ1 l1 l2 n) "Hσ1 /=". destruct σ1; simpl.
+    iIntros (σ1 l1 l2 n) "Hσ1 /=". destruct σ1 as [r0 m]; simpl.
     iDestruct "Hσ1" as "[Hr0 Hm]".
     assert (pc_p' ≠ O).
     { destruct pc_p'; auto. destruct pc_p; inversion Hfl. inversion Hvpc; naive_solver. }
@@ -64,7 +64,7 @@ Section cap_lang_rules.
   Proof.
     iIntros (Hinstr Hfl Hvpc ϕ) "(>HPC & >Hpc_a) Hφ".
     iApply wp_lift_atomic_head_step_no_fork; auto.
-    iIntros (σ1 l1 l2 n) "Hσ1 /=". destruct σ1; cbn.
+    iIntros (σ1 l1 l2 n) "Hσ1 /=". destruct σ1 as [r0 m]; cbn.
     iDestruct "Hσ1" as "[Hr0 Hm]".
     assert (pc_p' ≠ O).
     { destruct pc_p'; auto. destruct pc_p; inversion Hfl. inversion Hvpc; naive_solver. }
