theories/rules/rules_Jnz.v
@@ -9,10 +9,10 @@ Section cap_lang_rules.
   Context `{MachineParameters}.
   Implicit Types P Q : iProp Σ.
   Implicit Types σ : ExecConf.
-  Implicit Types c : cap_lang.expr. 
+  Implicit Types c : cap_lang.expr.
   Implicit Types a b : Addr.
   Implicit Types r : RegName.
-  Implicit Types v : cap_lang.val. 
+  Implicit Types v : cap_lang.val.
   Implicit Types w : Word.
   Implicit Types reg : gmap RegName Word.
   Implicit Types ms : gmap Addr Word.
@@ -51,7 +51,7 @@ Section cap_lang_rules.
   Proof.
     iIntros (Hinstr Hfl Hvpc HPC Dregs φ) "(>Hpc_a & >Hmap) Hφ".
     iApply wp_lift_atomic_head_step_no_fork; auto.
-    iIntros (σ1 l1 l2 n) "Hσ1 /=". destruct σ1; simpl.
+    iIntros (σ1 l1 l2 n) "Hσ1 /=". destruct σ1 as [r m]; simpl.
     iDestruct "Hσ1" as "[Hr Hm]".
     assert (pc_p' ≠ O).
     { destruct pc_p'; auto. destruct pc_p; inversion Hfl. inversion Hvpc; naive_solver. }
