theories/rules/rules_Lea.v
@@ -87,7 +87,7 @@ Section cap_lang_rules.
    Proof.
      iIntros (Hinstr Hfl Hvpc HPC Dregs φ) "(>Hpc_a & >Hmap) Hφ".
      iApply wp_lift_atomic_head_step_no_fork; auto.
-     iIntros (σ1 l1 l2 n) "Hσ1 /=". destruct σ1; simpl.
+     iIntros (σ1 l1 l2 n) "Hσ1 /=". destruct σ1 as [r m]; simpl.
      iDestruct "Hσ1" as "[Hr Hm]".
      assert (pc_p' ≠ O).
      { destruct pc_p'; auto. destruct pc_p; inversion Hfl. inversion Hvpc; naive_solver. }
