theories/rules/rules_LoadU.v
@@ -98,7 +98,7 @@ Section cap_lang_rules.
    Proof.
      iIntros (Hinstr Hfl Hvpc HPC Dregs Hmem_pc HaLoad φ) "(>Hmem & >Hmap) Hφ".
      iApply wp_lift_atomic_head_step_no_fork; auto.
-     iIntros (σ1 l1 l2 n) "[Hr Hm] /=". destruct σ1; simpl.
+     iIntros (σ1 l1 l2 n) "[Hr Hm] /=". destruct σ1 as [r m]; simpl.
      iDestruct (gen_heap_valid_inclSepM with "Hr Hmap") as %Hregs.
 
      (* Derive necessary register values in r *)
